src/Layer1.v
@@ -11,6 +11,8 @@ Section Layer1.
 
   Definition token_dec : forall (t t': token), {t=t'}+{t<>t'}. decide equality. Defined.
 
+  Definition oracle := list token.
+
   Definition state := disk (set value).
   
   Inductive prog : Type -> Type :=
@@ -20,44 +22,44 @@ Section Layer1.
   | Bind : forall T T', prog T -> (T -> prog T') -> prog T'.
    
   Inductive exec :
-    forall T, oracle token ->  state -> prog T -> @Result state T -> Prop :=
+    forall T, oracle ->  state -> prog T -> oracle -> @Result state T -> Prop :=
   | ExecRead : 
-      forall d a v,
+      forall o' d a v,
         read d a = Some v ->
-        exec [Cont] d (Read a) (Finished d v)
+        exec (Cont::o') d (Read a) o' (Finished d v)
              
   | ExecWrite :
-      forall d a v,
+      forall o' d a v,
         read d a <> None ->
-        exec [Cont] d (Write a v) (Finished (write d a v) tt)
+        exec (Cont::o') d (Write a v) o' (Finished (write d a v) tt)
              
   | ExecRet :
-      forall d T (v: T),
-        exec [Cont] d (Ret v) (Finished d v)
+      forall d T (v: T) o',
+        exec (Cont::o') d (Ret v) o' (Finished d v)
 
   | ExecBind :
       forall T T' (p1: prog T) (p2: T -> prog T')
-        o1 d1 d1' o2 r ret,
-        exec o1 d1 p1 (Finished d1' r) ->
-        exec o2 d1' (p2 r) ret ->
-        exec (o1++o2) d1 (Bind p1 p2) ret
+        o1 o1' d1 d1' o2 r ret,
+        exec o1 d1 p1 o1' (Finished d1' r) ->
+        exec o1' d1' (p2 r) o2 ret ->
+        exec o1 d1 (Bind p1 p2) o2 ret
 
   | ExecOpCrash :
-      forall T d (p: prog T),
+      forall T o' d (p: prog T),
         (forall T' (p1: prog T') p2, p <> Bind p1 p2) ->
-        exec [Crash] d p (Crashed d)
+        exec (Crash::o') d p o' (Crashed d)
              
   | ExecBindCrash :
       forall T T' (p1: prog T) (p2: T -> prog T')
-        o1 d1 d1',
-        exec o1 d1 p1 (Crashed d1') ->
-        exec o1 d1 (Bind p1 p2) (Crashed d1')
+        o1 o1' d1 d1',
+        exec o1 d1 p1 o1' (Crashed d1') ->
+        exec o1 d1 (Bind p1 p2) o1' (Crashed d1')
 
   | ExecBindFail :
       forall T T' (p1: prog T) (p2: T -> prog T')
-        o st st1,
-        exec o st p1 (Failed st1) ->
-        exec o st (Bind p1 p2) (Failed st1).
+        o o' st st1,
+        exec o st p1 o' (Failed st1) ->
+        exec o st (Bind p1 p2) o' (Failed st1).
   (* TODO: add Failed cases *)
   
 End Layer1.
