src/ProgAuto.v
@@ -9,7 +9,7 @@ Ltac invert_exec'' H :=
 
 Ltac invert_exec' :=
   match goal with
-  | [ H: exec _ _ ?p _ |- _ ] =>
+  | [ H: exec _ _ ?p _ _ |- _ ] =>
     match p with
     | Bind _ _ => idtac
     | Read _ => invert_exec'' H
@@ -19,26 +19,23 @@ Ltac invert_exec' :=
   end.
 
 Lemma bind_sep:
-  forall T T' o d (p1: prog T) (p2: T -> prog T') ret,
-    exec o d (Bind p1 p2) ret ->
+  forall T T' o o' d (p1: prog T) (p2: T -> prog T') ret,
+    exec o d (Bind p1 p2) o' ret ->
     match ret with
     | Finished d' r =>
-    (exists o1 o2 d1 r1,
-       exec o1 d p1 (Finished d1 r1) /\
-       exec o2 d1 (p2 r1) ret /\
-       o = o1++o2)
+    (exists o1 d1 r1,
+       exec o d p1 o1 (Finished d1 r1) /\
+       exec o1 d1 (p2 r1) o' ret)
   | Crashed d' =>
-    (exec o d p1 (Crashed d') \/
-     (exists o1 o2 d1 r1,
-        exec o1 d p1 (Finished d1 r1) /\
-        exec o2 d1 (p2 r1) ret /\
-        o = o1++o2))
+    (exec o d p1 o' (Crashed d') \/
+     (exists o1 d1 r1,
+        exec o d p1 o1 (Finished d1 r1) /\
+        exec o1 d1 (p2 r1) o' ret))
   | Failed d' =>
-    (exec o d p1 (Failed d') \/
-     (exists o1 o2 d1 r1,
-        exec o1 d p1 (Finished d1 r1) /\
-        exec o2 d1 (p2 r1) ret /\
-        o = o1++o2))
+    (exec o d p1 o' (Failed d') \/
+     (exists o1 d1 r1,
+        exec o d p1 o1 (Finished d1 r1) /\
+        exec o1 d1 (p2 r1) o' ret))
     end.
 Proof.
   intros.
@@ -52,16 +49,16 @@ Qed.
 
 Ltac invert_exec :=
   match goal with
-  |[H : exec _ _ (Bind _ _) _ |- _ ] =>
+  |[H : exec _ _ (Bind _ _) _ _ |- _ ] =>
    apply bind_sep in H; repeat cleanup
-  |[H : exec _ _ _ _ |- _ ] =>
+  |[H : exec _ _ _ _ _ |- _ ] =>
    invert_exec'
   end.
 
 
   Definition prog_equiv T : prog T -> prog T -> Prop :=
-    fun p1 p2 => forall o d out,
-        exec o d p1 out <-> exec o d p2 out.
+    fun p1 p2 => forall o o' d out,
+        exec o d p1 o' out <-> exec o d p2 o' out.
 
   Arguments prog_equiv {T} _ _.
 
@@ -70,54 +67,8 @@ Ltac invert_exec :=
   Theorem bind_assoc : forall T T' T'' (p1: prog T) (p2: T -> prog T') (p3: T' -> prog T''),
       Bind (Bind p1 p2) p3 ~= Bind p1 (fun x => Bind (p2 x) p3).
   Proof.
-    split; intros.
-    - repeat invert_exec; cleanup.
-      rewrite <- app_assoc.
-      repeat econstructor; eauto.
-
-      split_ors.
-      invert_exec; cleanup.
-      split_ors; cleanup.
-      eapply ExecBindCrash; auto.
-      
-      econstructor; eauto.
-      
-      invert_exec.
-      rewrite <- app_assoc.
-      repeat econstructor; eauto.
-
-      split_ors.
-      invert_exec; cleanup.
-      split_ors; cleanup.
-      eapply ExecBindFail; auto.
-      
-      econstructor; eauto.
-      
-      invert_exec.
-      rewrite <- app_assoc.
-      repeat econstructor; eauto.
-    
-    - repeat invert_exec; cleanup.
-      rewrite app_assoc.
-      repeat (eapply ExecBind; eauto).
-      
-      split_ors.
-      eapply ExecBindCrash; eauto.
-      
-      invert_exec.
-      split_ors.
-      eapply ExecBindCrash; eauto.
-      
-      rewrite app_assoc.
-      repeat econstructor; eauto.
-
-      split_ors.
-      eapply ExecBindFail; eauto.
-      
-      invert_exec.
-      split_ors.
-      eapply ExecBindFail; eauto.
-      
-      rewrite app_assoc.
-      repeat econstructor; eauto.
+    split; intros;
+      repeat invert_exec; cleanup;
+        repeat (split_ors; try invert_exec; cleanup);
+        intuition eauto.
   Qed.
